More progress...

src/mem/Addresses/InfiniteAddresses.v
@@ -8,7 +8,8 @@ From Vellvm Require Import
 
 From Mem Require Import
   Addresses.MemoryAddress
-  Memory.Provenance.
+  Memory.Provenance
+  Addresses.Provenance.
 
 From QuickChick Require Import Show.
 
@@ -30,10 +31,413 @@ Definition wildcard_prov : Prov := None.
 Definition nil_prov : Prov := Some [].
 
 (* TODO: If Prov is an NSet, I get a universe inconsistency here... *)
-Module InfAddr : MemoryAddress.ADDRESS
-with Definition addr := (Iptr * Prov) % type
+Module InfAddrType <: CORE_ADDRESS.
+  Definition t := (Iptr * Prov) % type.
+  Definition eq := @Logic.eq t.
+
+  (* TODO: is this what we should be using for equality on pointers? Probably *NOT* because of provenance. *)
+  Lemma eq_dec : forall (a b : t), {a = b} + {a <> b}.
+  Proof.
+    intros [a1 a2] [b1 b2].
+
+    destruct (Z.eq_dec a1 b1);
+      destruct (option_eq (fun x y => list_eq_dec N.eq_dec x y) a2 b2); subst.
+    - left; reflexivity.
+    - right. intros H. inversion H; subst. apply n. reflexivity.
+    - right. intros H. inversion H; subst. apply n. reflexivity.
+    - right. intros H. inversion H; subst. apply n. reflexivity.
+  Qed.
+
+  #[global] Instance eq_equiv : Equivalence eq.
+  typeclasses eauto.
+  Defined.
+End InfAddrType.
+
+Module InfNull <: HAS_NULL InfAddrType.
+  Definition null := (0, nil_prov)%Z.
+
+  Definition is_null (a : InfAddrType.t) : bool :=
+    Z.eqb (fst null) (fst a).
+
+  Lemma null_is_null :
+    is_null null = true.
+  Proof.
+    reflexivity.
+  Qed.
+End InfNull.
+
+Module InfPTOI <: HAS_PTOI InfAddrType.
+  Definition ptr_to_int := fun (ptr : InfAddrType.t) => fst ptr.
+End InfPTOI.
+
+Module Type Inf_HAS_POINTER_ARITHMETIC_CORE <: HAS_POINTER_ARITHMETIC_CORE InfAddrType.
+  (** Pointer addition. May error if the result cannot be represented
+      as a pointer, e.g., if it would be out of bounds.
+   *)
+  Definition ptr_add (a : InfAddrType.t) (i : Z) : err InfAddrType.t
+    := match a with
+       | (ptr, pr) =>
+           let res := ptr + i in
+           ret (res, pr)
+       end.
+
+  Lemma ptr_add_0 :
+    forall ptr,
+      ptr_add ptr 0 = inr ptr.
+  Proof.
+    intros ptr.
+    unfold ptr_add.
+    destruct ptr.
+    rewrite Z.add_0_r in *.
+    reflexivity.
+  Qed.
+End Inf_HAS_POINTER_ARITHMETIC_CORE.
+
+Module Type Inf_HAS_PROVENANCE <: HAS_PROVENANCE N_ProvSet InfAddrType.
+  Definition address_provenance := fun (ptr : InfAddrType.t) => snd ptr.
+End Inf_HAS_PROVENANCE.
+
+Module InfAddr <: ADDRESS := InfAddrType <+ InfNull <+ InfPTOI <+ Inf_HAS_POINTER_ARITHMETIC_CORE <+ HAS_POINTER_ARITHMETIC_HELPERS <+ Inf_HAS_PROVENANCE.
+
+Module FinPROV <: PROVENANCE(FinAddr)
+with Definition Prov := Prov
+with Definition address_provenance
+    := fun (a : FinAddr.addr) => snd a
+with Definition Provenance := Provenance
+with Definition AllocationId := AllocationId
+with Definition wildcard_prov := wildcard_prov
+with Definition nil_prov := nil_prov
+with Definition initial_provenance := 0%N
+with Definition provenance_to_prov := fun (pr : Provenance) => Some [pr]
+with Definition access_allowed := fun (pr : Prov) (aid : AllocationId)
+    => match pr with
+       | None => true (* Wildcard can access anything. *)
+       | Some prset =>
+         match aid with
+         | None => true (* Wildcard, can be accessed by anything. *)
+         | Some aid =>
+           existsb (N.eqb aid) prset
+         end
+       end.  
+
+  Definition Provenance := Provenance.
+  Definition AllocationId := AllocationId.
+  Definition Prov := Prov.
+  Definition wildcard_prov : Prov := wildcard_prov.
+  Definition nil_prov : Prov := nil_prov.
+  Definition address_provenance (a : FinAddr.addr) : Prov
+    := snd a.
+
+  (* Does the provenance set pr allow for access to aid? *)
+  Definition access_allowed (pr : Prov) (aid : AllocationId) : bool
+    := match pr with
+       | None => true (* Wildcard can access anything. *)
+       | Some prset =>
+         match aid with
+         | None => true (* Wildcard, can be accessed by anything. *)
+         | Some aid =>
+           existsb (N.eqb aid) prset
+         end
+       end.
+
+  Definition aid_access_allowed (pr : AllocationId) (aid : AllocationId) : bool
+    := match pr with
+       | None => true
+       | Some pr =>
+         match aid with
+         | None => true
+         | Some aid =>
+           N.eqb pr aid
+         end
+       end.
+
+  Definition allocation_id_to_prov (aid : AllocationId) : Prov
+    := fmap (fun x => [x]) aid.
+
+  Definition provenance_to_allocation_id (pr : Provenance) : AllocationId
+    := Some pr.
+
+  Definition provenance_to_prov (pr : Provenance) : Prov
+    := Some [pr].
+
+  Definition next_provenance (pr : Provenance) : Provenance
+    := N.succ pr.
+
+  Definition initial_provenance : Provenance
+    := 0%N.
+
+  Definition provenance_lt (p1 p2 : Provenance) : Prop
+    := N.lt p1 p2.
+
+  Lemma aid_access_allowed_refl :
+    forall aid, aid_access_allowed aid aid = true.
+  Proof.
+    intros aid.
+    unfold aid_access_allowed.
+    destruct aid; auto.
+    rewrite N.eqb_refl.
+    auto.
+  Qed.
+
+  Lemma access_allowed_refl :
+    forall aid,
+      access_allowed (allocation_id_to_prov aid) aid = true.
+  Proof.
+    intros aid.
+    unfold access_allowed.
+    cbn.
+    destruct aid; auto.
+    cbn.
+    rewrite N.eqb_refl.
+    cbn.
+    auto.
+  Qed.
+
+  Lemma allocation_id_to_prov_inv:
+    forall aid aid',
+      allocation_id_to_prov aid = allocation_id_to_prov aid' ->
+      aid = aid'.
+  Proof.
+    intros aid aid' H.
+    unfold allocation_id_to_prov in *.
+    cbn in *.
+    destruct aid, aid'; inv H; auto.
+  Qed.
+
+  Lemma provenance_to_allocation_id_inv :
+    forall pr pr',
+      provenance_to_allocation_id pr = provenance_to_allocation_id pr' ->
+      pr = pr'.
+  Proof.
+    intros pr pr' H.
+    unfold provenance_to_allocation_id in *.
+    inv H; auto.
+  Qed.
+
+  Lemma allocation_id_to_prov_provenance_to_allocation_id :
+    forall pr,
+      allocation_id_to_prov (provenance_to_allocation_id pr) = provenance_to_prov pr.
+  Proof.
+    intros pr.
+    cbn.
+    auto.
+  Qed.
+
+  Lemma provenance_eq_dec :
+    forall (pr pr' : Provenance),
+      {pr = pr'} + {pr <> pr'}.
+  Proof.
+    unfold Provenance.
+    unfold Provenance.Provenance.
+    intros pr pr'.
+    apply N.eq_dec.
+  Defined.
+
+  Lemma provenance_eq_dec_refl :
+    forall (pr : Provenance),
+      true = provenance_eq_dec pr pr.
+  Proof.
+    intros pr.
+    destruct provenance_eq_dec; cbn; auto.
+    exfalso; auto.
+  Qed.
+
+  Lemma aid_eq_dec :
+    forall (aid aid' : AllocationId),
+      {aid = aid'} + {aid <> aid'}.
+  Proof.
+    intros aid aid'.
+    destruct aid, aid'; auto.
+    pose proof provenance_eq_dec p p0.
+    destruct H; subst; auto.
+    right.
+    intros CONTRA. inv CONTRA; contradiction.
+    right; intros CONTRA; inv CONTRA.
+    right; intros CONTRA; inv CONTRA.
+  Qed.
+
+  Lemma aid_eq_dec_refl :
+    forall (aid : AllocationId),
+      true = aid_eq_dec aid aid.
+  Proof.
+    intros aid.
+    destruct (aid_eq_dec aid aid); cbn; auto.
+    exfalso; auto.
+  Qed.
+
+  #[global] Instance access_allowed_Proper :
+    Proper (eq ==> (fun aid aid' => true = (aid_eq_dec aid aid')) ==> eq) access_allowed.
+  Proof.
+    unfold Proper, respectful.
+    intros x y H x0 y0 H0.
+    subst.
+    unfold access_allowed.
+    symmetry in H0.
+    eapply proj_sumbool_true in H0.
+    subst.
+    reflexivity.
+  Defined.
+
+  #[global] Instance provenance_lt_trans : Transitive provenance_lt.
+  Proof.
+    unfold Transitive.
+    intros x y z XY YZ.
+    unfold provenance_lt in *.
+    lia.
+  Defined.
+
+  Lemma provenance_lt_next_provenance :
+    forall pr,
+      provenance_lt pr (next_provenance pr).
+  Proof.
+    unfold provenance_lt, next_provenance.
+    lia.
+  Qed.
+
+  Lemma provenance_lt_nrefl :
+    forall pr,
+      ~ provenance_lt pr pr.
+  Proof.
+    intros pr.
+    unfold provenance_lt.
+    lia.
+  Qed.
+
+  #[global] Instance provenance_lt_antisym : Antisymmetric Provenance eq provenance_lt.
+  Proof.
+    unfold Antisymmetric.
+    intros x y XY YX.
+    unfold provenance_lt in *.
+    lia.
+  Defined.
+
+  Lemma next_provenance_neq :
+    forall pr,
+      pr <> next_provenance pr.
+  Proof.
+    intros pr.
+    unfold next_provenance.
+    lia.
+  Qed.
+
+  Lemma access_allowed_aid_neq :
+    forall aid1 aid2,
+      aid1 <> aid2 ->
+      access_allowed
+        (allocation_id_to_prov (Some aid1)) (Some aid2) = false.
+  Proof.
+    intros aid1 aid2 NEQ.
+    unfold access_allowed.
+    unfold allocation_id_to_prov.
+    cbn.
+    rewrite orb_false_r.
+    eapply N.eqb_neq.
+    eauto.
+  Qed.
+
+  Lemma access_allowed_aid_eq :
+    forall aid1 aid2,
+      access_allowed
+        (allocation_id_to_prov (Some aid1)) (Some aid2) = true ->
+      aid1 = aid2.
+  Proof.
+    intros aid1 aid2 ACCESS.
+    unfold access_allowed, allocation_id_to_prov in *.
+    cbn in ACCESS.
+    rewrite orb_false_r in ACCESS.
+    eapply N.eqb_eq in ACCESS.
+    auto.
+  Qed.
+
+  (* Debug *)
+  Definition show_prov (pr : Prov) := Show.show pr.
+  Definition show_provenance (pr : Provenance) := Show.show pr.
+  Definition show_allocation_id (aid : AllocationId) := Show.show aid.
+End FinPROV.
+
+Module FinITOP : ITOP(FinAddr)(FinPROV)(FinPTOI)
+with Definition int_to_ptr :=
+  fun (i : Z) (pr : Prov) =>
+    if (i <? 0)%Z || (i >=? Int64.modulus)%Z
+    then Oom ("FinITOP.int_to_ptr: out of range (" ++ show i ++ ").")
+    else NoOom (Int64.repr i, pr).
+
+  Import FinAddr.
+  Import FinPROV.
+  Import FinPTOI.
+
+  Definition int_to_ptr (i : Z) (pr : Prov) : OOM addr
+    := if (i <? 0)%Z || (i >=? Int64.modulus)%Z
+       then Oom ("FinITOP.int_to_ptr: out of range (" ++ show i ++ ").")
+       else NoOom (Int64.repr i, pr).
+
+  Lemma int_to_ptr_provenance :
+    forall (x : Z) (p : Prov) (a : addr),
+      int_to_ptr x p = ret a ->
+      FinPROV.address_provenance a = p.
+  Proof.
+    intros x p a IP.
+    unfold int_to_ptr in *.
+    destruct ((x <? 0)%Z || (x >=? Int64.modulus)); inv IP; auto.
+  Qed.
+
+  Lemma int_to_ptr_ptr_to_int :
+    forall (a : addr) (p : Prov),
+      address_provenance a = p ->
+      int_to_ptr (ptr_to_int a) p = ret a.
+  Proof.
+    intros a p PROV.
+    unfold int_to_ptr.
+    unfold ptr_to_int.
+    destruct a; cbn.
+    pose proof Int64.unsigned_range i as R.
+    destruct ((Int64.unsigned i <? 0)%Z || (Int64.unsigned i >=? Int64.modulus)) eqn:RANGE; [lia|].
+    rewrite Int64.repr_unsigned.
+    inv PROV; cbn; auto.
+  Qed.
+
+  Lemma int_to_ptr_ptr_to_int_exists :
+    forall (a : addr) (p : Prov),
+    exists a',
+      int_to_ptr (ptr_to_int a) p = ret a' /\
+        ptr_to_int a' = ptr_to_int a /\
+        address_provenance a' = p.
+  Proof.
+    intros [a prov] p.
+    exists (a, p).
+    split; auto.
+    unfold int_to_ptr, ptr_to_int.
+    cbn in *.
+    destruct ((Int64.unsigned a <? 0)%Z || (Int64.unsigned a >=? Int64.modulus)) eqn:BOUNDS.
+    - (* Out of bounds *)
+      exfalso.
+      destruct a.
+      cbn in *.
+      lia.
+    - rewrite Int64.repr_unsigned.
+      reflexivity.
+  Qed.
+
+  Lemma ptr_to_int_int_to_ptr :
+    forall (x : Z) (p : Prov) (a : addr),
+      int_to_ptr x p = ret a ->
+      ptr_to_int a = x.
+  Proof.
+    intros x p a IP.
+    unfold int_to_ptr in *.
+    destruct ((x <? 0)%Z || (x >=? Int64.modulus)) eqn:RANGE; inv IP; auto.
+    unfold ptr_to_int. cbn.
+    rewrite Int64.unsigned_repr; auto.
+    unfold Int64.max_unsigned.
+    lia.
+  Qed.
+End FinITOP.
+
+
+Module InfAddr : MemoryAddress.INFINITE_ADDRESS
+with Definition t := (Iptr * Prov) % type
 with Definition null := (0, nil_prov)%Z.
-  Definition addr := (Iptr * Prov) % type.
+  Definition t := (Iptr * Prov) % type.
   Definition null : addr := (0, nil_prov)%Z.
 
   (* TODO: is this what we should be using for equality on pointers? Probably *NOT* because of provenance. *)
