src/mem/Semantics/Memory/Overlaps.v
@@ -18,7 +18,7 @@ Module Type Overlaps (Addr:MemoryAddress.ADDRESS).
 End Overlaps.
 
 (* Define overlapping of memory addresses when PTOI is defined. *)
-Module PTOIOverlaps (Addr:MemoryAddress.ADDRESS) (PTOI:PTOI(Addr)).
+Module PTOIOverlaps (Addr:MemoryAddress.ADDRESS) (PTOI:HAS_PTOI(Addr)).
   Import Addr.
   Import PTOI.
 
